\setcounter{section}{7}
\setcounter{exercise}{0}

\begin{exercise}
  \label{exercise:7.1}
  Probar que $\int_{a}^{b}d\alpha\left(x\right)=\alpha\left(b\right)-\alpha\left(a\right)$, directamente a partir de la definición de integral de Riemann-Stieltjes.
\end{exercise}

\begin{proof}

Sea $\text{\textepsilon}>0$ cualquiera. Tomemos $P_{\text{\textepsilon}}=\left\lbrace a,b\right\rbrace\in\mathcal{P}\left[a,b\right]$ y $f:\left[a,b\right]\text{\textrightarrow}\mathds{R}$ la función constante en $1$. Para cualquier $P\supseteq P_{\text{\textepsilon}}$ tenemos
\begin{align*}
  \left| S\left(P,f,\alpha\right)-\left(\alpha\left(b\right)-\alpha\left(a\right)\right)\right|&=\left|\left(\sum_{k=1}^{n}f\left(t_k\right)\Delta\alpha_k\right)-\left(\alpha\left(b\right)-\alpha\left(a\right)\right) \right|\\
  &=\left|\left(\sum_{k=1}^{n} \alpha\left(x_k\right)-\alpha\left(x_{k-1}\right)\right)-\left(\alpha\left(b\right)-\alpha\left(a\right)\right)\right|\\
  &=\left|\left(\alpha\left(b\right)-\alpha\left(a\right)\right)-\left(\alpha\left(b\right)-\alpha\left(a\right)\right)\right|\\
  &=0\\
  &<\text{\textepsilon},
\end{align*}
lo que prueba $\int_{a}^{b}d\alpha\left(x\right)=\alpha\left(b\right)-\alpha\left(a\right)$.
  
\end{proof}
